cleanup

Logic/MultiSuccCorsiTassi/Kripke.lean
@@ -17,7 +17,7 @@ def Seq4Proof.forced (s : Seq4Proof) : Finset Atom := s.as.toFinset
 
 def Seq4Proof.unforced (s : Seq4Proof) : Finset Atom := s.bs.toFinset
 
-def Seq4Proof.world (p : Seq4Proof) : World := ⟨p.forced, p.unforced \ p.forced⟩ -- , Finset.disjoint_sdiff⟩
+def Seq4Proof.world (p : Seq4Proof) : World := ⟨p.forced, p.unforced ⟩ -- , Finset.disjoint_sdiff⟩
 
 -- attribute [grind .] World.prop
 
@@ -153,16 +153,6 @@ termination_by fm m => (sizeOf_Form fm, m.depth)
 decreasing_by
 all_goals first | (apply Prod.Lex.left; grind) | (apply Prod.Lex.right; apply depth_lt_of_mem; grind)
 
-@[grind, simp]
-def impTrueCond (a b : Form) (m : Model) : Prop :=
-  ((a.eval m = TV.f ∨ b.eval m = TV.t)) ∧
-  (m.branch.all (λ m' => (a ⊃ b).eval m' = TV.t))
-
-@[grind, simp]
-def impFalseCond (a b : Form) (m : Model) : Prop :=
-  ((a.eval m = TV.t ∧ b.eval m = TV.f)) ∨
-  (m.branch.any (λ m' => (a ⊃ b).eval m' = TV.f))
-
 
 @[grind ., simp] theorem evalute_atom_t (h :  (Form.atoms a).eval m = .t) : a ∈ m.world.forced := by grind
 @[grind ., simp] theorem evalute_atom_f (h :  (Form.atoms a).eval m = .f) : a ∈ m.world.unforced := by grind
@@ -170,10 +160,7 @@ def impFalseCond (a b : Form) (m : Model) : Prop :=
 @[grind =, simp] theorem evalute_bot : Form.bot.eval m = .f := by grind
 @[grind =, simp] theorem evalute_and : (a ∧∧ b).eval m = conjTV (a.eval m) (b.eval m) := by grind
 @[grind =, simp] theorem evalute_or : (a ∨∨ b).eval m = disjTV (a.eval m) (b.eval m) := by grind
-@[grind =, simp]
-theorem evalute_atom_undef :
-    (Form.atoms a).eval m = .u ↔ a ∉ m.world.forced ∧ a ∉ m.world.unforced := by
-  grind
+@[grind =, simp] theorem evalute_atom_undef : (Form.atoms a).eval m = .u ↔ a ∉ m.world.forced ∧ a ∉ m.world.unforced := by grind
 
 
 /- def evalBlocked : Imp → Model → TV
@@ -185,12 +172,10 @@ theorem evalute_atom_undef :
 
 def evalAnt (Γ : Multiset Form) (m : Model) : TV :=
   (Γ.map (fun f => f.eval m)).fold conjTV TV.t
-
 scoped notation "⋀ " m:max ", " Γ:max => evalAnt Γ m
 
 def evalSucc (Δ : Multiset Form) (m : Model) : TV :=
   (Δ.map (fun f => f.eval m)).fold disjTV TV.f
-
 scoped notation "⋁ " m:max ", " Γ:max => evalSucc Γ m
 
 -- A sequent is refutable iff all its assumptions are satisfied (all forms in Γ are true) but none of the conclusions are (all Δ are false)
@@ -255,31 +240,12 @@ lemma evalSucc_not_f (h : x ∈ ys) (hx : x.eval m = .u) : ¬⋁ m, ys = TV.f :=
     · simp_all [evalSucc]
     · simp_all [evalSucc]
 
-@[grind =, simp]
-lemma evalSucc_bot_cons : ⋁ m, ↑(⊥ :: xs) = ⋁ m, ↑xs := by
-  simp [evalSucc]
-
-@[grind =, simp]
-lemma evalAnt_bot_cons : ⋀ m, ↑(⊥ :: xs) = .f := by
-  simp [evalAnt]
-
-@[grind =, simp]
-lemma evalAnt_conj : ⋀ m, ↑((a ∧∧ b) :: xs) = ⋀ m, ↑(a :: b :: xs) := by
-  simp [evalAnt]; grind
-
-@[grind =, simp]
-lemma evalSucc_conj : ⋁ m, ↑((a ∨∨ b) :: xs) = ⋁ m, ↑(a :: b :: xs) := by
-  simp [evalSucc]; grind
-
-@[grind =, simp]
-lemma evalSucc_cons {xs : List Form} :
-    ⋁ m, ↑(a :: xs) = disjTV (a.eval m) (⋁ m, ↑xs) := by
-  simp [evalSucc]
-
-@[grind =, simp]
-lemma evalAnt_cons {xs : List Form} :
-    ⋀ m, ↑(a :: xs) = conjTV (a.eval m) (⋀ m, ↑xs) := by
-  simp [evalAnt]
+@[grind =, simp] lemma evalSucc_bot_cons : ⋁ m, ↑(⊥ :: xs) = ⋁ m, ↑xs := by simp [evalSucc]
+@[grind =, simp] lemma evalAnt_bot_cons : ⋀ m, ↑(⊥ :: xs) = .f := by simp [evalAnt]
+@[grind =, simp] lemma evalAnt_conj : ⋀ m, ↑((a ∧∧ b) :: xs) = ⋀ m, ↑(a :: b :: xs) := by simp [evalAnt]; grind
+@[grind =, simp] lemma evalSucc_conj : ⋁ m, ↑((a ∨∨ b) :: xs) = ⋁ m, ↑(a :: b :: xs) := by simp [evalSucc]; grind
+@[grind =, simp] lemma evalSucc_cons {xs : List Form} : ⋁ m, ↑(a :: xs) = disjTV (a.eval m) (⋁ m, ↑xs) := by simp [evalSucc]
+@[grind =, simp] lemma evalAnt_cons {xs : List Form} : ⋀ m, ↑(a :: xs) = conjTV (a.eval m) (⋀ m, ↑xs) := by simp [evalAnt]
 
 @[grind =, simp]
 lemma evalAnt_eq_true :
@@ -289,7 +255,6 @@ lemma evalAnt_eq_true :
 lemma evalAnt_eq_false :
     ⋀ m, xs = .f ↔ ∃ x ∈ xs, x.eval m = .f := by
   induction xs using Multiset.induction with simp_all [evalAnt]
-
 @[grind =, simp]
 lemma evalSucc_eq_true :
     ⋁ m, xs = .t ↔ ∃ x ∈ xs, x.eval m = .t := by
@@ -298,7 +263,6 @@ lemma evalSucc_eq_true :
 lemma evalSucc_eq_false :
     ⋁ m, xs = .f ↔ ∀ x ∈ xs, x.eval m = .f := by
   induction xs using Multiset.induction with simp_all [evalSucc]
-
 @[grind ., simp]
 lemma evalSucc_true (fin : f ∈ Δ ) (ev : f.eval m = TV.t ): evalSucc Δ m = TV.t := by
  simp; grind
@@ -307,111 +271,42 @@ lemma evalAnt_false (h₁ : f ∈ Γ) (h₂ : f.eval m = TV.f) : evalAnt Γ m = 
   simp; grind
 
 
-lemma eval_if_else_false {a b : Form} :
-  ((if ((a.eval m = TV.f) ∨ (b.eval m = TV.t)) ∧ ∀ x ∈ m.branch, ((a ⊃ b).eval x = TV.t) then TV.t
-  else if (a.eval m = TV.t) ∧ (b.eval m = TV.f) ∨ ∃ x ∈ m.branch, ((a ⊃ b).eval x = TV.f) then TV.f
-  else TV.u) =
-  TV.f) → (a.eval m = TV.t) ∧ (b.eval m = TV.f) ∨ ∃ x ∈ m.branch, ((a ⊃ b).eval x = TV.f) := by
-  intro h
-  split_ifs at h
-  . grind
-
-
-
-lemma eval_if_else_true {a b : Form}
-  (ifss : ((if ((a.eval m = TV.f) ∨ (b.eval m = TV.t)) ∧ ∀ x ∈ m.branch, ((a ⊃ b).eval x = TV.t) then TV.t
-  else if (a.eval m = TV.t) ∧ (b.eval m = TV.f) ∨ ∃ x ∈ m.branch, ((a ⊃ b).eval x = TV.f) then TV.f
-  else TV.u) =
-  TV.t)) : ((a.eval m = TV.f) ∨ (b.eval m = TV.t)) ∧ ∀ x ∈ m.branch, ((f ⊃ g).eval x = TV.t) := by
-
-
-  sorry
-
 
 --IMP EVAL--
-@[grind =, simp]
-theorem eval_imp_false_local :
-  a.eval m = .t → b.eval m = .f → (a ⊃ b).eval m = .f  := by
-  intro h₁ h₂; rw [Form.eval]; rw [h₁, h₂] ; simp
+theorem eval_imp_true_iff :
+  (a ⊃ b).eval m = TV.t ↔
+    ((a.eval m = .f ∨ b.eval m = .t) ∧ (m.branch.all (λ m' => (a ⊃ b).eval m' = .t))) := by
+  constructor
+  . intro h; rw [Form.eval] at h; simp_all; grind [Form.eval]
+  . intro h; rw [Form.eval]; simp_all
 
-@[grind =, simp]
-theorem eval_imp_true_if {a b : Form} : ((a.eval m = .f ∨ b.eval m = .t)
-      ∧ (m.branch.all (λ m' => (a ⊃ b).eval m' = .t))) → (a ⊃ b).eval m = .t := by grind [Form.eval]
+theorem eval_imp_false_iff :
+  (a ⊃ b).eval m = TV.f ↔
+    a.eval m = .t ∧  b.eval m = .f ∨ ∃ x ∈ m.branch, ((a ⊃ b).eval x = TV.f) := by
+  constructor
+  . intro h; rw [Form.eval] at h; simp_all
+    split_ifs at h
+    . grind
+  . intro h; rw [Form.eval]; simp_all; grind
 
-@[grind =, simp]
-theorem eval_imp_true_orl {a b : Form} {m : Model} :
-  (a.eval m = .f /- ∨ g.eval m = .t -/) → (m.branch.all (λ m' => (a ⊃ b).eval m' = .t)) → (a ⊃ b).eval m = .t := by
-  intro h₁ h₂
-  rw [Form.eval]; simp_all
-
-@[grind =, simp]
-theorem eval_imp_true_orr {a b : Form} :
-  (b.eval m = .t) → (m.branch.all (λ m' => (a ⊃ b).eval m' = .t)) → (a ⊃ b).eval m = .t := by
-  intro h₁ h₂
-  rw [Form.eval]; simp_all
-
--- IN USE
---@[grind ., simp]
-theorem eval_imp_true_then (h₁ : (a ⊃ b).eval m = .t) :
-  (a.eval m = .f ∨ b.eval m = .t)
-      ∧ (m.branch.all (λ m' => (a ⊃ b).eval m' = .t)) := by
-  rw [Form.eval] at h₁; simp_all; grind [Form.eval]
-
-
-
---@[grind ., simp]
-theorem eval_imp_false_then :
-  (a ⊃ b).eval m = TV.f → a.eval m = .t ∧  b.eval m = .f ∨ ∃ x ∈ m.branch, ((a ⊃ b).eval x = TV.f) := by
-    intro h;
-    rw [Form.eval] at h
-    simp_all
-    apply eval_if_else_false at h
-    exact h
-
---@[grind ., simp]
-theorem eval_imp_false_if {a b : Form} {m : Model}
-(h : (a.eval m = .t ∧  b.eval m = .f) ∨ (∃ x ∈ m.branch, ((a ⊃ b).eval x = TV.f))) :
-  (a ⊃ b).eval m = TV.f := by
-  rw [Form.eval];
-  simp_all
-  grind
-
-
--- IN USE
 theorem eval_imp_righ_wo_ys :
   evalSeq { Γ := ↑xs, Δ := {a ⊃ b} } m ≠ TV.f →
   evalSeq { Γ := ↑xs, Δ := ↑((a ⊃ b) :: ys) } m ≠ TV.f := by
   simp; intro h₁ h₂; simp_all
 
--- IN USE
--- TODO CHANGE TO IFF?? TODO changed to .branch not .all. Thoughts?
 @[grind ., simp]
 theorem eval_imp_false_contradict :
   (a ⊃ b).eval m = TV.f → ∃ m' ∈ m.all, a.eval m' = .t ∧ b.eval m' = .f := by
   intro impF
   fun_induction Model.all with
   | case1 m ih =>
-    apply eval_imp_false_then at impF
+    rw [eval_imp_false_iff] at impF
     rcases impF with impF | ⟨m', impF⟩
     . grind
     . simp_all
       specialize ih m' (by grind) impF.right
       obtain ⟨m'', ih⟩ := ih
       grind
-
-/- @[grind ., simp]
-theorem eval_imp_false_iff :
-  (a ⊃ b).eval m = TV.f ↔ ∃ m' ∈ m.branch, a.eval m' = .t ∧ b.eval m' = .f := by
-  constructor
-  . intro h
-    apply eval_imp_false_then at h
-    rcases h with impF | ⟨m', impF⟩
-
-  . intro h
-    rcases h with ⟨m', h₁, h₂, h₃⟩
-    apply eval_imp_false_if
-    right
-    grind -/
 
 
 --MONOTONICITY--
@@ -422,16 +317,12 @@ theorem mono_true_form {a : Form} {m : Model} :
   ( a.eval m = .t) → (∀ x ∈ m.branch, a.eval x = .t)  := by sorry -/
 
 @[grind ., simp]
-theorem branch_mem_of_all {m m' a : Model} (h₁ : a ∈ m.branch) (h₂ : m' ∈ a.all) : m' ∈ m.all := by
+theorem Model.all_nested_in_all {m m' a : Model} (h₁ : a ∈ m.branch) (h₂ : m' ∈ a.all) : m' ∈ m.all := by
   fun_induction Model.all m with
-  | case1 m ih =>
-    simp_all
-    right
-    grind
+  | case1 m ih => simp_all; right; grind
 
--- IN USE
 @[grind ., simp]
-theorem wf_of_mem_all {m m' : Model} (wf : m.wf) (mem : m' ∈ m.all) : m'.wf := by
+theorem Model.all_wf {m m' : Model} (wf : m.wf) (mem : m' ∈ m.all) : m'.wf := by
   fun_induction Model.all with
   | case1 m ih =>
     simp_all
@@ -443,7 +334,7 @@ theorem wf_of_mem_all {m m' : Model} (wf : m.wf) (mem : m' ∈ m.all) : m'.wf :=
 
 --TODO IMPORTANT
 @[grind ., simp]
-theorem model_branch_mono_t {f : Form} {m m' : Model}
+theorem Model.momo_branch_true {f : Form} {m m' : Model}
   (wf : m.wf) (mem : m' ∈ m.branch) (ftv : f.eval m = TV.t) :
     f.eval m' = TV.t := by
   have h : ∀ a ∈ m.branch, a.wf = true ∧
@@ -459,29 +350,29 @@ theorem model_branch_mono_t {f : Form} {m m' : Model}
     simp_all
     constructor
     . obtain ⟨atv, btv⟩ := ftv
-      apply model_branch_mono_t wf mem
+      apply Model.momo_branch_true wf mem
       exact atv
     . obtain ⟨atv, btv⟩ := ftv
-      apply model_branch_mono_t wf mem
+      apply Model.momo_branch_true wf mem
       exact btv
   | .or a b =>
     simp_all
     cases ftv with
     | inl h =>
       left
-      apply model_branch_mono_t wf mem
+      apply Model.momo_branch_true wf mem
       exact h
     | inr h =>
       right
-      apply model_branch_mono_t wf mem
+      apply Model.momo_branch_true wf mem
       exact h
   | .imp a b =>
-    apply eval_imp_true_then at ftv
+    rw [eval_imp_true_iff] at ftv
     obtain ⟨h₁, h₂⟩ := ftv
     grind
 
 -- IN USE
-theorem model_all_mono {f : Form} {m m' : Model}
+theorem Model.mono_all_true {f : Form} {m m' : Model}
   (wf : m.wf) (mem : m' ∈ m.all) (ftv : f.eval m = TV.t) :
   f.eval m' = TV.t := by
   rw [Model.all] at mem
@@ -489,24 +380,17 @@ theorem model_all_mono {f : Form} {m m' : Model}
   simp_all
   rcases mem with h | ⟨a, h₁, h₂⟩
   . grind
-  . have wf' : m'.wf = true := wf_of_mem_all wf (by grind)
-    have aT := model_branch_mono_t wf h₁ ftv
+  . have wf' : m'.wf = true := Model.all_wf wf (by grind)
+    have aT := Model.momo_branch_true wf h₁ ftv
     have awf : a.wf := by
       rw [Model.wf] at wf; simp at wf
       grind
-    apply model_all_mono awf h₂ aT
+    apply Model.mono_all_true awf h₂ aT
 termination_by (m.depth)
 decreasing_by exact depth_lt_of_mem h₁
 
-
--- IN USE
 @[grind ., simp]
-theorem model_all_mono_list {xs : List Form} {m m' : Model}
-  (wf : m.wf) (mem : m' ∈ m.all) (xstv : ∀ x ∈ xs, x.eval m = TV.t) :
-  ∀ x ∈ xs, x.eval m' = TV.t := by grind [model_all_mono]
-
-@[grind ., simp]
-theorem mono_false_form_branch {f : Form} {m m' : Model}
+theorem Model.mono_branch_false {f : Form} {m m' : Model}
   (wf : m.wf) (mem : m' ∈ m.branch ) (ftv : f.eval m' = .f) :
   f.eval m = .f  := by
   have h : ∀ a ∈ m.branch, a.wf = true ∧
@@ -524,23 +408,23 @@ theorem mono_false_form_branch {f : Form} {m m' : Model}
     cases ftv with
     | inl h =>
       left
-      apply mono_false_form_branch wf mem
+      apply Model.mono_branch_false wf mem
       exact h
     | inr h =>
       right
-      apply mono_false_form_branch wf mem
+      apply Model.mono_branch_false wf mem
       exact h
   | .or a b =>
     simp_all
     constructor
     . obtain ⟨atv, btv⟩ := ftv
-      apply mono_false_form_branch wf mem
+      apply Model.mono_branch_false wf mem
       exact atv
     . obtain ⟨atv, btv⟩ := ftv
-      apply mono_false_form_branch wf mem
+      apply Model.mono_branch_false wf mem
       exact btv
   | .imp a b =>
-    apply eval_imp_false_if
+    rw [eval_imp_false_iff]
     right
     use m'
 
@@ -553,7 +437,7 @@ theorem mono_false_form_branch {f : Form} {m m' : Model}
   . have awf : a.wf = true := by rw [Model.wf] at wf; simp at wf; grind
     have mmwf : mm.wf = true := by rw [Model.wf] at awf; simp at awf; grind
     sorry
-    --have : f.eval mm = .f := mono_false_form_branch mmwf mem ftv
+    --have : f.eval mm = .f := Model.mono_branch_false mmwf mem ftv
     --exact mono_false_all_branch (by sorry) h₁ h₂
 
 
@@ -565,55 +449,28 @@ theorem mono_false_form_all {f : Form} {m m' : Model}
   rcases mem with h | ⟨a, h₁, h₂⟩
   . grind
   . have h := mono_false_all_branch wf h₁ h₂ ftv
-    have wf' : m'.wf = true := wf_of_mem_all wf (by grind)
-    exact mono_false_form_branch wf h₁ h -/
+    have wf' : m'.wf = true := Model.all_wf wf (by grind)
+    exact Model.mono_branch_false wf h₁ h -/
 
 
-theorem imo_branch_false_then_b_false {a b : Form} {m m' : Model}
+theorem imp_false_branch {a b : Form} {m m' : Model}
 (mem : m' ∈ m.branch) (h : (a ⊃ b).eval m' = TV.f) (wf : m.wf) :
 b.eval m = TV.f := by
-  apply eval_imp_false_then at h
+  rw [eval_imp_false_iff] at h
   rcases h with ⟨atv, btv⟩ | h
-  . exact mono_false_form_branch wf mem btv
+  . exact Model.mono_branch_false wf mem btv
   . obtain ⟨x, xmem, h⟩ := h
     have mwf : m'.wf = true := by rw [Model.wf] at wf; simp at wf; grind
-    have := imo_branch_false_then_b_false xmem h mwf
-    exact mono_false_form_branch wf mem this
+    have := imp_false_branch xmem h mwf
+    exact Model.mono_branch_false wf mem this
 termination_by (m.depth)
 decreasing_by exact depth_lt_of_mem mem
 
 -- IN USE
-theorem eval_imp_false_then_b_false  (impF : (a ⊃ b).eval m = TV.f) (wf : m.wf) : b.eval m = .f := by
-  apply eval_imp_false_then at impF
+theorem imp_false_then_b_false  (impF : (a ⊃ b).eval m = TV.f) (wf : m.wf) : b.eval m = .f := by
+  rw [eval_imp_false_iff] at impF
   cases impF with
   | inl h => grind
   | inr h =>
     rcases h with ⟨m', mem, h₂⟩
-    exact imo_branch_false_then_b_false mem h₂ wf
-
-
-
-/- theorem Model_monotonicity_t {m: Model} : ∀ fm ∈ m.branch, m.world.forced ⊆ fm.world.forced := by sorry
-theorem Model_monotonicity_f {m: Model} : ∀ fm ∈ m.branch, fm.world.unforced ⊆ m.world.unforced := by sorry
- -/
-/-
-@[simp]
-theorem eval_imp_false_future {m : Model} {h : m.wf} {a b : Form}:
-  (∃ x ∈ m.branch, ((a ⊃ b).eval x = TV.f)) →
-  (a ⊃ b).eval m = .f := by
-  sorry -/
-
-/- @[grind ., simp]
-theorem eval_imp_not_false_then :
-  (¬(a ⊃ b).eval m = TV.f) →
-  impTrueCond a b m ∨ (¬ impTrueCond a b m ∧ ¬ impFalseCond a b m) := by
-  intro h; rw [Form.eval] at h; simp at h
-  by_cases hT :
-  ((a.eval m = TV.f) ∨ (b.eval m = TV.t)) ∧
-  ∀ x ∈ m.branch, ((a ⊃ b).eval x = TV.t)
-  · left
-    exact hT
-  · right
-    constructor
-    · intro hT'; grind
-    · sorry -/
+    exact imp_false_branch mem h₂ wf
